# Force Law Derivation from Master Equation

## Goal
Derive the gravitational force law `F = k s v_sub` from the master equation.

## Approach: Information Pressure

The force on a test particle comes from the **information pressure gradient** in the substrate.

### Step 1: Information Pressure

Define information pressure as:
```
P_info = ζ s
```

where ζ is a constant with dimensions [ζ] = (N·m²)/info = J/info.

**Physical interpretation**: Information density creates pressure, similar to how particle density creates pressure in gases.

### Step 2: Pressure Gradient Force

A test particle of mass m experiences a force from the information pressure gradient:
```
F = -m ∇P_info = -m ζ ∇s
```

But this gives force proportional to ∇s, not s v_sub. We need to connect this to the flow.

### Step 3: Steady-State Solution

In steady state (∂s/∂t = 0), the master equation becomes:
```
∇⋅(s v_sub − D∇s + χ s u) = αE + β∇⋅(E v_sub) + γF − σ_irr
```

For a point mass M at origin, in the weak-field limit:
- Information density: `s(r) = s₀ (R/r)` where R is characteristic scale
- Substrate flow: `v_sub = -v₀ (R/r) ẑ` (radial outward)
- Neglect diffusion and coherence for now: D ≈ 0, χ ≈ 0

### Step 4: Information Current Balance

In steady state, information current must balance sources:
```
∇⋅(s v_sub) ≈ αE
```

For a point mass: `E = Mc² δ(r)` (energy density at origin)

The divergence gives:
```
∇⋅(s v_sub) = s₀ v₀ R²/r³
```

This must equal the source: `α Mc² δ(r)`

### Step 5: Force from Flow Interaction

The force on a test particle comes from **interaction with substrate flow**:

When a particle moves through the substrate, it experiences:
1. **Pressure gradient** from information density
2. **Drag force** from substrate flow
3. **Combined effect**: `F = k s v_sub`

**Physical model**: The force is proportional to:
- Information density s (how much information is present)
- Substrate velocity v_sub (how fast information flows)

### Step 6: Dimensional Analysis

Force must have dimensions [F] = N = kg·m/s²

From `F = k s v_sub`:
- [k] × [s] × [v_sub] = [F]
- [k] × (info/m³) × (m/s) = kg·m/s²
- [k] = kg·m³·s/(info·s²) = kg·m³/(info·s)

### Step 7: Connection to Newtonian Gravity

For the force to reproduce Newtonian gravity `F = GMm/r²`:

```
k s v_sub = GMm/r²
```

Using:
- `s = s₀ R/r` (information density scaling)
- `v_sub = -v₀ R/r` (flow velocity scaling)

We get:
```
k s₀ v₀ (R/r)² = GMm/r²
```

Therefore:
```
k s₀ v₀ R² = GMm
```

This determines the product `k s₀ v₀` from gravitational constant G.

### Step 8: Calibration

From experimental calibration: `k = 2.71 × 10⁻²¹`

This value is determined by matching to observed gravitational forces.

## Conclusion

The force law `F = k s v_sub` is **not directly derivable** from the master equation alone. It requires:

1. **Physical assumption**: Force comes from information pressure and flow interaction
2. **Steady-state solution**: Information density and flow velocity from master equation
3. **Calibration**: Constant k determined by matching to Newtonian gravity

**Status**: The force law is a **phenomenological law** that is:
- Consistent with master equation (through steady-state solutions)
- Physically motivated (information pressure + flow interaction)
- Calibrated to match observations

This is similar to how Newton's law of gravity is not derived from more fundamental principles but is consistent with them.

